\paragraph*{Claim}

Every member of the version space lies between $G$ and $S$, i.$\,$e.,

\[
h\in\mathit{VS}_{\mathcal{H},E}\Rightarrow\exists\, g\in G,\, s\in S:g\leq h\leq s
\]
where
\[
g\in G\Leftrightarrow\left(g\text{ consistent with }E\right)\land\left(\forall h\in\mathcal{H}:h<g\Rightarrow h\text{ is inconsistent with }E\right)
\]
\[
s\in S\Leftrightarrow\left(s\text{ consistent with }E\right)\land\left(\forall h\in\mathcal{H}:s<h\Rightarrow h\text{ is inconsistent with }E\right)
\]



\paragraph*{Proof by contrapositive}

The contrapositive of the claim is
\[
\lnot\left(\exists\, g\in G,\, s\in S:g\leq h\leq s\right)\Rightarrow\lnot\left(h\in\mathit{VS}_{\mathcal{H},E}\right)
\]
which is identical to 
\[
\nexists\, g\in G,\, s\in S:g\leq h\leq s\Rightarrow h\not\in\mathit{VS}_{\mathcal{H},E}.
\]
Using the definition for the set $G$
\[
\begin{aligned}G & =\left\{ g\in\mathit{VS}_{\mathcal{H},E}\mid\forall h\in\mathcal{H}:h<g\Rightarrow h\text{ is inconsistent with }E\right\} \\
 & =\left\{ g\in\mathit{VS}_{\mathcal{H},E}\mid\forall h\in\mathcal{H}:h<g\Rightarrow h\not\in\mathit{VS}_{\mathcal{H},E}\right\} \\
 & =\left\{ g\in\mathit{VS}_{\mathcal{H},E}\mid g\leq h\;\forall h\in\mathit{VS}_{\mathcal{H},E}\right\} 
\end{aligned}
\]
we arrive at 
\[
\nexists\, g\in G:g\text{\ensuremath{\leq}}h\Rightarrow h\not\in\mathit{VS}_{\mathcal{H},E}.
\]
Similarly, for the set $S$
\[
\begin{aligned}S & =\left\{ s\in\mathit{VS}_{\mathcal{H},E}\mid\forall h\in\mathcal{H}:s<h\Rightarrow h\text{ is inconsistent with }E\right\} \\
 & =\left\{ s\in\mathit{VS}_{\mathcal{H},E}\mid\forall h\in\mathcal{H}:s<h\Rightarrow h\not\in\mathit{VS}_{\mathcal{H},E}\right\} \\
 & =\left\{ s\in\mathit{VS}_{\mathcal{H},E}\mid h\leq s\;\forall h\in\mathit{VS}_{\mathcal{H},E}\right\} 
\end{aligned}
\]
we obtain
\[
\nexists\, s\in S:h\leq s\Rightarrow h\not\in\mathit{VS}_{\mathcal{H},E}.
\]
Thus, 
\[
\nexists\, g\in G,\, s\in S:g\leq h\leq s\Rightarrow h\not\in\mathit{VS}_{\mathcal{H},E}
\]
 which proofs that the contrapositive of the claim and therefore the
claim itself are true. \newline \phantom{x}\hfill $\blacksquare$
